Concrete.ec added

proof/SomeDKC.ec
@@ -1,5 +1,5 @@
 require import Int.
-require import IntExtra.
+require import IntDiv.
 require import Bool.
 require import Real.
 require import NewFMap.
@@ -7,6 +7,7 @@ require import FSet.
 require import Distr.
 require import Option.
 require import Array.
+require import Pair.
 
 require (*--*) SomePRF.
 require (*--*) DKC.
@@ -37,7 +38,7 @@ theory SomeDKC.
         op E = E,
         op D = D.
 
-  prover ["Z3"].
+  (*prover ["Z3"].*)
         
   (** DKC security definitions, instantiated with the words defined in W *)
   clone import DKCSec2.DKCSecurity with
@@ -56,7 +57,7 @@ theory SomeDKC.
       game; otherwise, we are in a OTP world, because tweaks do not
       repeat. *)
    
-  op bound: int.
+  (*op bound: int.*)
     
   module Param = {
     var kpub : ((int * bool), (KW.word * bool)) fmap
@@ -66,17 +67,33 @@ theory SomeDKC.
     var tbl : (word,word) fmap
   }.
 
-  op kw2w(kw,lsb) = if kw = witness
-                    then witness
-                    else let lsbi = if lsb then 1 else 0
+  op kw2w(kw,lsb) =
+                   let lsbi = if lsb then 1 else 0
                       in let kwi = (KW.to_int kw) * 2 + lsbi
                       in W.from_int kwi.
 
-    op w2kw(w) = if w = witness
-                    then witness
-                    else let kwi = (W.to_int w) (* / 2 *)
+  op kw2w'(kw,lsb) =
+  if kw = witness then witness else
+  let lsbi = if lsb then 1 else 0
+                      in let kwi = (KW.to_int kw) * 2 + lsbi
+    in W.setlsb (W.from_int kwi) lsb.
+
+
+
+    
+
+  op w2kw(w) =
+  if w = witness then witness else
+  let kwi = (W.to_int w) %/ 2 (* / 2 *)
                           in let lsbi = W.getlsb w
                           in (KW.from_int kwi,lsbi).
+
+  op w2kw'(w) =
+  if w = witness then witness else
+  let kwi = (W.to_int w) %/ 2 (* / 2 *)
+                          in let lsbi = W.getlsb w
+                          in KW.from_int kwi.
+  
     
   module DKC_Oracle(O:PRF_Oracle) = {
     proc encrypt(q:query_DKC) : answer_DKC = {
@@ -105,7 +122,7 @@ theory SomeDKC.
                         then (ki, witness) 
                         else (ki,kj));
 
-        xx = let (kxx,lsbxx) = oget Param.kpub.[lb] in kw2w kxx lsbxx;
+        xx = let (kxx,lsbxx) = oget Param.kpub.[lb] in kw2w' kxx lsbxx;
 
         if (rn) {
           xx = $Dword.dword;
@@ -113,15 +130,15 @@ theory SomeDKC.
         
         if ((Param.l,Param.lsb)=ib) {
           mask = O.f(t);
-          ans = (kw2w ki lsbi, kw2w kj lsbj, mask ^ (F kj t) ^ xx);
+          ans = (kw2w' ki lsbi, kw2w' kj lsbj, mask ^ (F kj t) ^ xx);
         }
         else  {
             if ((Param.l,Param.lsb)=jb) {
               mask = O.f(t);
-              ans = (kw2w ki lsbi, kw2w kj lsbj, (F ki t) ^ mask ^ xx);
+              ans = (kw2w' ki lsbi, kw2w' kj lsbj, (F ki t) ^ mask ^ xx);
            }
            else  {
-              ans = (kw2w ki lsbi, kw2w kj lsbj, (F ki t) ^ (F kj t) ^ xx);
+              ans = (kw2w' ki lsbi, kw2w' kj lsbj, (F ki t) ^ (F kj t) ^ xx);
            }
         }
       }
@@ -146,7 +163,7 @@ theory SomeDKC.
       i = 0;
       while (i < bound) {
         Param.kpub.[(i, false)] = (KW.zeros,false);
-        Param.kpub.[(i, true)] = (KW.zeros,false);
+        Param.kpub.[(i, true)] = (KW.zeros,true);
         i = i + 1;
       }
 
@@ -178,14 +195,49 @@ theory SomeDKC.
       return adv;
     }
   }.
-
-
+      
+  
 equiv true_key l b (A <:  Adv_DKC_t):
     DKCSecurity.Game(DKC,A).game ~
-    IND(PRFr_Wrapped,D(A)).main : 0 <= l{1} < bound && b{1} = true
+    IND(PRFr_Wrapped,D(A)).main : 0 <= l < boundl /\ b = true
                                ==> ={res}.
     proof.
-      proc. inline DKC.initialize PRFr_Wrapped.init D(A,PRFr_Wrapped).distinguish.
+      proc.
+      inline PRFr_Wrapped.init D(A,PRFr_Wrapped).distinguish. print W.
+      seq 1 3 : (0 <= l < boundl /\ b = true /\
+      DKCp.used{1} = Param.used{2} /\ DKCp.used{1} = fset0 /\
+      DKCp.l{1} = Param.l{2} /\
+      DKCp.lsb{1} = Param.lsb{2} /\
+      Param.tbl{2} = map0 /\
+      (forall k, 0 <= k < bound => oget DKCp.kpub{1}.[(k,true)] = kw2w' (fst (oget Param.kpub{2}.[(k,true)])) true) /\
+      (forall k, 0 <= k < bound => oget DKCp.kpub{1}.[(k,false)] = kw2w' (fst (oget Param.kpub{2}.[(k,false)])) false) /\
+      (forall k, 0 <= k < bound => getlsb (oget DKCp.kpub{1}.[(k,true)]) = snd (oget Param.kpub{2}.[(k,true)])) /\
+      (forall k, 0 <= k < bound => getlsb (oget DKCp.kpub{1}.[(k,false)]) = snd (oget Param.kpub{2}.[(k,false)])));   
+      inline DKC.initialize D(A, PRFr_Wrapped).initialize.
+    
+        wp; while (0 <= l < boundl /\ b = true /\ ={i} /\ 0 <= i{1} <= bound /\
+      DKCp.used{1} = Param.used{2} /\ DKCp.used{1} = fset0 /\
+      DKCp.l{1} = Param.l{2} /\
+      DKCp.lsb{1} = Param.lsb{2} /\
+      Param.tbl{2} = map0 /\
+      (forall k, 0 <= k < i{1} => oget DKCp.kpub{1}.[(k,true)] = kw2w' (fst (oget Param.kpub{2}.[(k,true)])) true) /\
+      (forall k, 0 <= k < i{1} => oget DKCp.kpub{1}.[(k,false)] = kw2w' (fst (oget Param.kpub{2}.[(k,false)])) false) /\
+      (forall k, 0 <= k < i{1} => getlsb (oget DKCp.kpub{1}.[(k,true)]) = snd (oget Param.kpub{2}.[(k,true)])) /\
+      (forall k, 0 <= k < i{1} => getlsb (oget DKCp.kpub{1}.[(k,false)]) = snd (oget Param.kpub{2}.[(k,false)]))).
+        
+        if; first by progress. print w2kw.
+        wp. rnd (fun w, w2kw w) (fun w, kw2w' w (!Param.lsb{2})). wp. rnd{1}. rnd. skip; progress.
+        by rewrite Dword.dwordLsb_lossless.
+        simplify w2kw kw2w' fst. case (kiR = witness) => hc. smt tmo=15. 
+        rewrite KW.Dword.mu_x_def Dword.dwordLsb_mu_x. cut ->: getlsb (kw2w' kiR (!lsbL)) = !lsbL <=> true. simplify kw2w'. rewrite get_setlsb. done. done.
+        by smt.
+        simplify w2kw kw2w' fst; smt tmo=15. 
+        idtac=>/#.
+        idtac=>/#.
+        rewrite !getP. case (k = Param.l{2}) => hc. case (true = !lsbL) => hc'. rewrite hc hc' //. cut ->: (k, true) = (Param.l{2}, !lsbL) <=> false by idtac=>/#. cut ->: (k, true) = (Param.l{2}, lsbL) <=> true by idtac=>/#. simplify. rewrite oget_some. simplify kw2w'. rewrite oget_some. simplify fst => /#. case ((k, true) = (Param.l{2}, lsbL)) => hc'. rewrite oget_some. simplify kw2w'. rewrite oget_some. simplify fst. => /#. cut ->: (k, true) = (Param.l{2}, lsbL) <=> false. simplify. by. idtac=>/#. rewrite oget_some. simplify kw2w'. rewrite oget_some. simplify fst => /#. 
+    
+
+    
       admit.
     qed.
 
