proof/Concrete.ec
@@ -1,0 +1,677 @@
+require import Real.
+require import Int.
+require import Pair.
+require import Array.
+
+require        SFE.
+require        EffSch.
+require        ProjSch.
+require        SomeOT.
+require        Prot.
+require        ProtSec.
+
+import ArrayExt.
+
+theory Concrete.
+  clone import ExtWord as W.
+  clone import SomeOT.SomeOT with
+    theory WS <- W.
+  clone import EffSch.EfficientScheme as ES with
+    theory W <- W.
+  
+   (* Definition of leakage for both PFE and SFE protocols *)
+   op pfe_or_sfe : bool.
+
+   import ES.ProjScheme.
+   
+   op sch_phi (fn:Sch.Scheme.fun_t): Sch.Scheme.fun_t=
+    if pfe_or_sfe
+     then (* PFE: leaks the circuit's topology *)
+          ( fst fn,
+           map (fun x, (false,false,false,false)) (snd fn))
+     else (* SFE: circuit is public *) fn.
+
+   op leakInterface (x: Sch.Scheme.fun_t * int) : Sch.Scheme.leak_t * int = 
+          let (n, m, q, aa, bb) = fst (fst x) in
+          (Sch.Scheme.phi (fst x), n - (snd x)).
+
+   type state1_t = SomeOT.st_c_t.
+   type rand1_t = SomeOT.OTSecurity.OT.rand1_t.
+   type state2_t = SomeOT.st_s_t * Sch.Scheme.funG_t  * Sch.Scheme.outputK_t * 
+                     word array * SomeOT.rand2_s_t.
+   type rand2_t = SomeOT.OTSecurity.OT.rand2_t * Sch.Scheme.rand_t.
+  
+   type msg1_t = SomeOT.msg1_t.
+   type msg2_t = SomeOT.msg2_t.
+   type msg3_t = SomeOT.msg3_t * Sch.Scheme.funG_t * Sch.Scheme.outputK_t * 
+                 word array.
+   type conv_t = msg1_t * msg2_t * msg3_t.
+   
+   op p1_stage1 (i1:bool array) (r1:rand1_t) (m1:msg1_t): state1_t * msg2_t  =
+     SomeOT.msg2 i1 r1 m1.
+   
+   op p1_stage2 (st:state1_t) (m3:msg3_t): Sch.Scheme.output_t =
+     let (ot_msg_in,fg_in,ko_in,x2g_in) = m3 in
+     let ot_out = SomeOT.result st ot_msg_in in
+     let outG = Sch.Scheme.evalG fg_in (ot_out || x2g_in) in
+         Sch.Scheme.decode ko_in outG.
+
+   op p2_stage1 (i2:Sch.Scheme.fun_t * bool array) (r2:rand2_t): state2_t * msg1_t = 
+      let (fn,x2) = i2 in
+      let (r_ot,r_s) = r2 in
+      let (n,m,q,a,b) = fst fn in 
+      let r_f = ES.Local.randFormat (n+q) m r_s in
+      let fg = ES.Local.funG fn r_f in (* Not calling Scheme functions, for efficiency *)
+      let ki = ES.Local.inputK fn r_f in  (* Not calling Scheme functions, for efficiency *)
+      let ko = ES.Local.outputK fn r_f in  (* Not calling Scheme functions, for efficiency *)
+      let x2g = Sch.Scheme.Input.encode 
+                  (drop (n - size (snd i2)) ki) x2 in
+      let (st_ot,m1) = SomeOT.msg1 
+                  (take (n - size (snd i2)) ki) (fst r_ot) in
+          ((st_ot,fg,ko,x2g,snd r_ot) , m1).
+
+   op p2_stage2 (st:state2_t) (m2:msg2_t): msg3_t  = 
+      let (st_ot,fg,ko,x2g,r_ot2) = st in
+      let m3 = SomeOT.msg3 st_ot r_ot2 m2 in
+          (m3,fg,ko,x2g).
+end Concrete.
+import Concrete.
+import ES.ProjScheme.
+(*********************************
+  Correctness and Security proofs
+**********************************)
+
+  (* summarises the concrete protocol *)
+  op conc_prot (i1 :bool array) (r1:rand1_t)
+               (i2:Sch.Scheme.fun_t * bool array) (r2:rand2_t) : conv_t* (Sch.Scheme.output_t * unit) =
+    let (st2, m1) = p2_stage1 i2 r2 in
+    let (st1, m2) = p1_stage1 i1 r1 m1 in
+    let m3 = p2_stage2 st2 m2 in
+    let outcome = p1_stage2 st1 m3 in
+    ((m1, m2, m3), (outcome, ())).
+
+  clone ProtSec.ProtSecurity with 
+    type Protocol.rand1_t = rand1_t,
+    type Protocol.input1_t = bool array,
+    type Protocol.output1_t = Sch.Scheme.output_t,
+    type Protocol.leak1_t = int,
+    type Protocol.rand2_t = rand2_t,
+    type Protocol.input2_t = Sch.Scheme.fun_t * bool array,
+    type Protocol.output2_t = unit,
+    op Protocol.f (i1: input1_t, i2: input2_t) =
+         (Sch.Scheme.eval (fst i2) (i1 || snd i2), ()),
+    type Protocol.leak2_t = Sch.Scheme.fun_t * int,
+    type Protocol.conv_t = conv_t,
+    op Protocol.validInputs(i1: input1_t, i2: input2_t) =
+       let (fg,x2) = i2 in
+       0 < size i1 /\ Sch.Scheme.validInputs fg (i1||x2),
+    pred Protocol.validRands(i1: input1_t, i2: input2_t, r1: rand1_t, r2: rand2_t) =
+       let (fg,x2) = i2 in
+       Sch.Scheme.validRand fg (snd r2),
+    op Protocol.prot = conc_prot,
+    op Protocol.phi1 = SomeOT.OTSecurity.OTPSec.Protocol.phi1,
+    op Protocol.phi2 (i2:input2_t) = (sch_phi (fst i2), size (snd i2)).
+
+    print Sch.Scheme.fun_t.
+
+    print SFE.SFE.
+    
+  clone SFE.SFE as CSFE with
+    type ProjScheme.token_t = W.word,
+    (* Scheme *)
+    type ProjScheme.Sch.Scheme.fun_t = ES.ProjScheme.Sch.Scheme.fun_t,
+    type ProjScheme.Sch.Scheme.funG_t = ES.ProjScheme.Sch.Scheme.funG_t,
+    type ProjScheme.Sch.Scheme.output_t = ES.ProjScheme.Sch.Scheme.output_t,
+    type ProjScheme.Sch.Scheme.outputK_t = ES.ProjScheme.Sch.Scheme.outputK_t,
+    type ProjScheme.Sch.Scheme.outputG_t = ES.ProjScheme.Sch.Scheme.outputG_t,
+    type ProjScheme.Sch.Scheme.leak_t = ES.ProjScheme.Sch.Scheme.leak_t,
+    type ProjScheme.Sch.Scheme.rand_t = ES.ProjScheme.Sch.Scheme.rand_t,
+    pred ProjScheme.Sch.Scheme.validRand = ES.ProjScheme.Sch.Scheme.validRand,
+    op ProjScheme.Sch.Scheme.validInputs = ES.ProjScheme.Sch.Scheme.validInputs,
+    op ProjScheme.Sch.Scheme.phi = ES.ProjScheme.Sch.Scheme.phi,
+    op ProjScheme.Sch.Scheme.eval = ES.ProjScheme.Sch.Scheme.eval,
+    op ProjScheme.Sch.Scheme.funG = ES.ProjScheme.Sch.Scheme.funG,
+    op ProjScheme.Sch.Scheme.inputK = ES.ProjScheme.Sch.Scheme.inputK,
+    op ProjScheme.Sch.Scheme.outputK = ES.ProjScheme.Sch.Scheme.outputK,
+    op ProjScheme.Sch.Scheme.decode = ES.ProjScheme.Sch.Scheme.decode,
+    op ProjScheme.Sch.Scheme.evalG = ES.ProjScheme.Sch.Scheme.evalG,
+    op ProjScheme.Sch.Scheme.pi_sampler = ES.ProjScheme.Sch.Scheme.pi_sampler,
+    (* OT *)
+    type ot_rand1_t = SomeOT.OTSecurity.OT.rand1_t,
+    type ot_rand2_t = SomeOT.OTSecurity.OT.rand2_t,
+    type ot_conv_t = SomeOT.OTSecurity.OT.conv_t,
+    op ot_prot = SomeOT.OTSecurity.OT.prot,
+    op sfe_sch_phi = sch_phi,
+    op leakInterface = leakInterface.
+    
+ (* Correctness *)
+
+ lemma phi_sch_phi (fn: Sch.Scheme.fun_t) :
+  Sch.Scheme.phi (sch_phi fn) = Sch.Scheme.phi fn.
+ proof strict. rewrite /sch_phi; case pfe_or_sfe; smt. qed.
+
+ lemma length_inputK fn r:
+  let (n, m, q, aa, bb) = fst fn in
+  0 < n =>
+  0 <= q =>
+  size (Sch.Scheme.inputK fn r) = n.
+ proof strict. 
+   simplify fst. 
+   rewrite /Sch.Scheme.inputK /ES.Local.inputK /fst //.
+   elim fn.`1 => n m q aa bb hn hq. simplify.
+   
+ rewrite /= size_sub //; first smt.
+ rewrite /ES.Local.randFormat.
+ cut Hr: size r < n + q
+         \/ (size r < n +q)=false by smt.
+ elim Hr => Hr; rewrite Hr //=.
+ rewrite size_offun; smt. 
+ rewrite size_mapi; smt.
+ qed.
+
+ lemma compatible :
+  CSFE.Compatibility ().
+ proof strict.
+ delta CSFE.Compatibility CSFE.ProtSecurity.Protocol.validInputs => /= i1 i2 [H1].
+  rewrite /CSFE.ProjScheme.Sch.Scheme.validInputs /Sch.Scheme.validInputs
+          /Sch.Scheme.validInputs /ES.Local.validInputs.
+  elim i2=> fn2 xx2 /=.
+  elim fn2=> tt2 gg2 /=.
+  elim tt2=> n m q aa bb /=.
+  rewrite /ES.Local.validCircuit.
+  simplify fst snd.
+  rewrite size_append => /= [[H2] [H3 H4]].
+  split; rewrite /CSFE.leakInterface /leakInterface
+     /CSFE.ProtSecurity.Protocol.phi2 /CSFE.sfe_sch_phi !/fst !/snd /=; first smt.
+  split;simplify delta.
+    by case pfe_or_sfe; smt.
+    move=> r; case (size r < n + q)=> lenr_nq.
+      rewrite size_sub //=; first smt.
+      by rewrite size_mkarray; smt.
+      rewrite size_sub //=; first smt.
+      by rewrite size_mapi; smt.
+ qed.
+
+ (* bijection between concrete and abstract PFE/SFE protocol views *) 
+ op conv_trl (sfe_conv:CSFE.ProtSecurity.Protocol.conv_t)
+ : ProtSecurity.Protocol.conv_t =
+  let (fg,x2g,oK) = fst sfe_conv in
+  let (otm1,otm2,otm3) =  snd sfe_conv in
+  (otm1,otm2,(otm3,fg,oK,x2g)).
+
+ lemma prot_trl: forall i1 r1 i2 r2,
+  CSFE.ProtSecurity.Protocol.validInputs i1 i2 =>
+  (*let r2' = (let (r21, r22) = r2 in let (n, m, q, aa, bb) = fst (fst i2) in (r21, ES.Local.randFormat (n + q)%Int m r22)) in*)
+  ProtSecurity.Protocol.prot i1 r1 i2 r2
+  = ( conv_trl (fst (CSFE.ProtSecurity.Protocol.prot i1 r1 i2 r2))
+    , snd (CSFE.ProtSecurity.Protocol.prot i1 r1 i2 r2)).
+ proof strict. 
+move => i1 r1 i2 r2.
+   elim r2=> r21 r22 /=.
+   elim i2=> fn x /=.
+   elim fn=> topo gg /=.
+   elim topo=> n m q aa bb /=.
+   move => Hvalid.
+   cut Hcompat: CSFE.Compatibility () by apply compatible.
+   move : Hcompat; rewrite /CSFE.Compatibility => Hcompat.
+   elim (Hcompat i1 (((n,m,q,aa,bb),gg),x) _); first smt.
+   move=> {Hcompat} Hleak1 [Hleak2] HlenIK.
+   move : Hvalid;
+   rewrite /CSFE.ProtSecurity.Protocol.validInputs /CSFE.ProtSecurity.Protocol.validInputs
+    /CSFE.ProjScheme.Sch.Scheme.validInputs /Sch.Scheme.validInputs /Sch.Scheme.validInputs /Sch.Scheme.validInputs /ES.Local.validInputs size_append /=
+    => [[H1] [H2 H3]].
+   rewrite /ProtSecurity.Protocol.prot /conc_prot.
+   rewrite /conc_prot /p2_stage1 /p2_stage2 /p1_stage1 /p1_stage2.
+   rewrite /CSFE.ProtSecurity.Protocol.prot /CSFE.ProtSecurity.Protocol.prot
+    /CSFE.OTSecurity.OT.prot /SomeOT.OTSecurity.OT.prot /SomeOT.ot_prot /=
+    /CSFE.OTSecurity.OTPSec.Protocol.prot /CSFE.OTSecurity.OT.prot
+    /CSFE.OTSecurity.OT.prot /CSFE.ot_prot /SomeOT.OTSecurity.OT.prot /SomeOT.ot_prot ! fst_pair ! snd_pair /=.
+   pose sm1 := (SomeOT.msg1 _ _); rewrite (pairS sm1) /=.
+   pose sm2 := (SomeOT.msg2 _ _ _); rewrite (pairS sm2) /=.
+   pose sm3 := (SomeOT.msg3 _ _ _); rewrite (pairS sm3) /=.
+   pose sm1' := (SomeOT.msg1 _ _); rewrite (pairS sm1') /=.
+   pose sm2' := (SomeOT.msg2 _ _ _); rewrite (pairS sm2') /=.
+   pose sm3' := (SomeOT.msg3 _ _ _); rewrite (pairS sm3') /=.
+   cut -> : sm1 = sm1' by smt.
+   cut -> : sm2 = sm2' by smt.
+   cut -> : sm3 = sm3' by smt.
+   cut ->: (CSFE.ProjScheme.Sch.Scheme.decode = Sch.Scheme.decode) by trivial.
+ cut ->: (CSFE.ProjScheme.Sch.Scheme.evalG = Sch.Scheme.evalG) by trivial.
+ cut ->: (CSFE.ProjScheme.Sch.Scheme.Input.encode = Sch.Scheme.Input.encode) by trivial.
+ cut ->: (CSFE.ProjScheme.Sch.Scheme.funG = Sch.Scheme.funG) by trivial.
+ cut ->: (CSFE.ProjScheme.Sch.Scheme.outputK = Sch.Scheme.outputK) by trivial.
+ cut ->: (CSFE.ProjScheme.Sch.Scheme.inputK = Sch.Scheme.inputK) by trivial.
+ cut -> : n - size x = size i1 by smt.
+ do ! (split=> //).
+ qed.
+
+ print CSFE.ProjScheme.Sch.Scheme.Correct.
+ 
+
+ 
+ lemma Correctness:  ES.SomeGarble.DKCSecurity.D.Correct () =>
+  ProtSecurity.Correct (). 
+ proof strict.
+  (*move => DKCh.
+  rewrite /ProtSecurity.Correct /ProtSecurity.Protocol.validInputs => i1 r1 i2 r2.
+   simplify Sch.Scheme.validInputs ES.Local.validInputs.
+   simplify ProtSecurity.Protocol.f.  move => H H1.
+   rewrite (pairS i2) /=.
+  rewrite prot_trl /CSFE.ProtSecurity.Protocol.validInputs.
+    /CSFE.ProtSecurity.Protocol.validInputs /CSFE.ProjScheme.Sch.Scheme.validInputs /Sch.Scheme.validInputs !snd_pair ?fst_pair.
+   split. smt. move : H2. simplify Sch.Scheme.validInputs. simplify ES.Local.validInputs. smt.
+  cut ->: ProtSecurity.Protocol.f = CSFE.ProtSecurity.Protocol.f by trivial.
+  apply CSFE.PFE_Correctness.
+   by apply compatible.
+   by cut:= ES.sch_correct _ => //.
+   by apply OT.ot_correct.
+   by smt.
+   generalize vRands.
+   simplify ProtSecurity.Protocol.validRands CSFE.ProtSecurity.Protocol.validRands CSFE.ProtSecurity.Protocol.validRands CSFE.ProjScheme.Sch.Scheme.validRand Sch.Scheme.validRand ES.ProjScheme.Sch.Scheme.validRand.
+   by rewrite !/fst /=.*) admit.
+ qed.
+
+ (* Security *)
+
+ module R1 = CSFE.PFE_R1(SomeOT.R1).
+ print CSFE.PFE_R2.
+ print ES.SomeGarble.Rand.
+ print ES.SomeGarble.tokens_t.
+ 
+ print CSFE.SchSecurity.EncSecurity.Encryption.rand.
+ print CSFE.ProjScheme.Sch.Scheme.rand_t.
+ print Sch.Scheme.rand_t.
+
+
+ module R2 = CSFE.PFE_R2(SomeOT.R2, ES.Rand). 
+ module SFESim = CSFE.PFE_S(ES.Rand,ES.SchSecurity.EncSecurity.SIM(ES.Rand),SomeOT.S).
+
+ module S : ProtSecurity.Sim_t = {
+  proc sim1(i1 : ProtSecurity.Protocol.input1_t,
+           o1 : ProtSecurity.Protocol.output1_t,
+           l2 : ProtSecurity.Protocol.leak2_t) : ProtSecurity.view1_t = {
+   var sfe_view : CSFE.ProtSecurity.view1_t;
+     
+   sfe_view = SFESim.sim1(i1,o1,l2);
+   return (fst sfe_view,conv_trl (snd sfe_view));
+  }
+
+  proc sim2(i2 : ProtSecurity.Protocol.input2_t,
+           o2 : ProtSecurity.Protocol.output2_t,
+           l1 : ProtSecurity.Protocol.leak1_t) : ProtSecurity.view2_t = {
+   var sfe_view : CSFE.ProtSecurity.view2_t;
+
+   sfe_view = SFESim.sim2(i2,o2,l1);
+   return (fst sfe_view,conv_trl (snd sfe_view));
+  }
+ }.
+
+ module SFE_A1(A1 : ProtSecurity.Adv1_t) : CSFE.ProtSecurity.Adv1_t = {
+  proc gen_query()
+  : CSFE.ProtSecurity.Protocol.input1_t*CSFE.ProtSecurity.Protocol.input2_t = {
+   var query: ProtSecurity.Protocol.input1_t*ProtSecurity.Protocol.input2_t;
+   query =  A1.gen_query();
+   return query;
+  }
+
+  proc dist (view: CSFE.ProtSecurity.view1_t) : bool = {
+   var guess: bool;
+   guess = A1.dist((fst view, conv_trl(snd view)));
+   return guess;
+  }        
+ }.
+
+ module SFE_A2(A2 : ProtSecurity.Adv2_t) : CSFE.ProtSecurity.Adv2_t = {
+  proc gen_query()
+  : CSFE.ProtSecurity.Protocol.input1_t*CSFE.ProtSecurity.Protocol.input2_t={
+   var query: ProtSecurity.Protocol.input1_t*ProtSecurity.Protocol.input2_t;
+   query =  A2.gen_query();
+   return query;
+  }
+  proc dist (view: CSFE.ProtSecurity.view2_t) : bool = {
+   var guess: bool;
+   guess = A2.dist((fst view, conv_trl(snd view)));
+   return guess;
+  }
+ }.
+
+ lemma Connect_SFE_1 : 
+  forall (A1 <: ProtSecurity.Adv1_t) &m,
+   islossless A1.gen_query =>
+   islossless A1.dist =>
+   equiv [ ProtSecurity.Game1(R1, R2, S, A1).main ~
+           CSFE.ProtSecurity.Game1(R1, R2, SFESim, SFE_A1(A1)).main : 
+          ={glob A1} ==> ={res} ].
+ proof strict.
+ move => A1 &m A1genll A1distll. proc => //.
+   inline ProtSecurity.Game1(CSFE.PFE_R1(SomeOT.R1), CSFE.PFE_R2(SomeOT.R2, ES.Rand), S, A1).game.
+   inline CSFE.ProtSecurity.Game1(CSFE.PFE_R1(SomeOT.R1), CSFE.PFE_R2(SomeOT.R2, ES.Rand), CSFE.PFE_S(ES.Rand, ES.SchSecurity.EncSecurity.SIM(ES.Rand), SomeOT.S), SFE_A1(A1)).game.
+ seq 3 3 : (={i1,i2,glob A1,b} /\ real{1} = real{2} /\ b{1} = real{1}).
+   inline SFE_A1(A1).gen_query.
+  wp.
+  call (_ : ={glob A1} ==> ={glob A1,res}); first by proc true.
+   wp; rnd.
+
+   by skip. 
+   case (! ProtSecurity.Protocol.validInputs i1{1} i2{1}).
+  rcondt {1} 1; first by move => &m0; skip.
+  rcondt {2} 1; first by move => &m0; skip; smt.
+  by wp; rnd; skip. 
+ rcondf {1} 1; first by move => &m0; skip; smt.
+ rcondf {2} 1.
+  move => &m0; skip; progress; move : H.
+  rewrite /ProtSecurity.Protocol.validInputs (pairS i2{hr}) /=.
+  by simplify Sch.Scheme.validInputs.
+  admit.
+  smt.
+ case (real{1}).
+  rcondt {1} 1; first by move => &m0; skip.
+  rcondt {2} 1; first by move => &m0; skip.
+  inline SFE_A1(A1).dist.
+  wp; call (_ :  ={glob A1,view} ==> ={res}); first by proc true.
+  wp; call (_ : ={i2info} ==> ={res}).
+   by proc; call ES.Rand_stateless; call SomeOT.R2_stateless; skip.
+  call (_ : ={i1info} ==> ={res}).
+   by proc; call SomeOT.R1_stateless; skip.
+  skip;progress;
+  rewrite snd_pair prot_trl; move : H; 
+  rewrite /ProtSecurity.Protocol.validInputs
+    /CSFE.ProtSecurity.Protocol.validInputs
+    /CSFE.ProjScheme.Sch.Scheme.validInputs. admit. smt.
+ rcondf {1} 1; first by move => &m0; skip.
+ rcondf {2} 1; first by move => &m0; skip.
+ inline SFE_A1(A1).dist.
+ wp; call (_ :  ={glob A1,view} ==> ={res}); first by proc true.
+ inline S.sim1 SFESim.sim1.
+ inline CSFE.PFE_S(ES.Rand, ES.SchSecurity.EncSecurity.SIM(ES.Rand), SomeOT.S).sim1.
+ wp; call SomeOT.S1_stateless; call ES.Sim_stateless.
+ wp; skip; progress; smt.
+ qed.
+
+ lemma Connect_SFE_1_pr : 
+  forall (A1 <: ProtSecurity.Adv1_t) &m,
+   islossless A1.gen_query =>
+   islossless A1.dist =>
+   Pr[ProtSecurity.Game1(R1, R2, S, A1).main() @ &m : res] = 
+   Pr[CSFE.ProtSecurity.Game1(R1, R2, SFESim, SFE_A1(A1)).main() @ &m : res].
+ proof strict.
+ move => A1 &m A1genll A1getll.
+ byequiv (Connect_SFE_1 A1 &m _ _) => //.
+ qed.
+
+ lemma Connect_SFE_2 : 
+  forall (A2 <: ProtSecurity.Adv2_t) &m,
+    islossless A2.gen_query =>
+    islossless A2.dist =>
+    equiv [ ProtSecurity.Game2(R1, R2, S, A2).main ~
+            CSFE.ProtSecurity.Game2(R1, R2, SFESim, SFE_A2(A2)).main : 
+            ={glob A2} ==> ={res} ].
+ proof strict.
+ move => A2 &m A2genll A2getll; proc.
+ inline ProtSecurity.Game2(CSFE.PFE_R1(SomeOT.R1), CSFE.PFE_R2(SomeOT.R2, ES.Rand), S, A2).game.
+ inline CSFE.ProtSecurity.Game2(CSFE.PFE_R1(SomeOT.R1), CSFE.PFE_R2(SomeOT.R2, ES.Rand), CSFE.PFE_S(ES.Rand, ES.SchSecurity.EncSecurity.SIM(ES.Rand), SomeOT.S), SFE_A2(A2)).game.
+   seq 3 3 : (={glob A2,i1,i2,b} /\ real{1} = real{2} /\ b{1} = real{1}).
+ inline SFE_A2(A2).gen_query. 
+  wp; call (_ : ={glob A2} ==> ={glob A2,res}); first by proc true.
+  wp; rnd; skip; progress; smt.
+ case (ProtSecurity.Protocol.validInputs i1{1} i2{1}).
+  rcondf {1} 1; first by move => &m0; skip; smt.
+  rcondf {2} 1.
+   move => &m0;skip;move => &hr; progress; move : H;
+   rewrite /ProtSecurity.Protocol.validInputs (pairS i2{hr}) /=; admit.
+  case (real{1}).
+   rcondt {1} 1; first by move => &m0; skip; smt.
+   rcondt {2} 1; first by move => &m0; skip; smt.
+   inline SFE_A2(A2).dist.
+   wp; call (_ : ={glob A2,view} ==> ={glob A2,res}); first by proc true.
+   wp; inline CSFE.PFE_R2(SomeOT.R2, ES.Rand).gen.
+   wp; call ES.Rand_stateless; call SomeOT.R2_stateless.
+   wp; inline CSFE.PFE_R1(SomeOT.R1).gen.
+   wp; call (_ : ={i1info} ==> ={res}); first by proc; rnd; wp; skip.
+   wp; skip; progress; rewrite snd_pair prot_trl; move : H;
+   rewrite /ProtSecurity.Protocol.validInputs
+    /CSFE.ProtSecurity.Protocol.validInputs
+    /CSFE.ProjScheme.Sch.Scheme.validInputs; admit.
+  rcondf {1} 1; first by move => &m0; skip.
+  rcondf {2} 1; first by move => &m0; skip.
+  inline SFE_A2(A2).dist.
+  wp;call (_ :  ={glob A2,view} ==> ={res}); first by proc true.
+  inline S.sim2 SFESim.sim2.
+  inline CSFE.PFE_S(ES.Rand, ES.SchSecurity.EncSecurity.SIM(ES.Rand), SomeOT.S).sim2.
+  wp; call SomeOT.S2_stateless; call ES.Rand_stateless.
+  wp; skip; progress; smt.
+ rcondt {1} 1; first by move => &m0; skip.
+ rcondt {2} 1; first by move => &m0; skip; smt.
+ by wp; rnd; skip.
+ qed.
+
+ lemma Connect_SFE_2_pr : 
+  forall (A2 <: ProtSecurity.Adv2_t) &m,
+    islossless A2.gen_query =>
+    islossless A2.dist =>
+     Pr[ProtSecurity.Game2(R1, R2, S, A2).main() @ &m : res] = 
+       Pr[CSFE.ProtSecurity.Game2(R1, R2, SFESim, SFE_A2(A2)).main() @ &m : res].
+ proof strict.
+ move => A2 &m A2genll A2getll.
+ by byequiv (Connect_SFE_2 A2 &m _ _).
+ qed.
+
+ lemma Connect_SomeOT_1 : 
+  forall (A1 <: CSFE.OTSecurity.OTPSec.Adv1_t) &m,
+    islossless A1.gen_query =>
+    islossless A1.dist =>
+    equiv [ CSFE.OTSecurity.OTPSec.Game1(SomeOT.R1, SomeOT.R2, SomeOT.S, A1).main ~
+            SomeOT.OTSecurity.OTPSec.Game1(SomeOT.R1, SomeOT.R2, SomeOT.S, A1).main : 
+            ={glob A1} ==> ={res} ].
+ proof strict.
+ move => A1 &m A1genll A1distll; proc.
+  inline CSFE.OTSecurity.OTPSec.Game1(SomeOT.R1, SomeOT.R2, SomeOT.S, A1).game.
+  inline SomeOT.OTSecurity.OTPSec.Game1(SomeOT.R1, SomeOT.R2, SomeOT.S, A1).game.
+   seq 3 3 : (={i1,i2,glob A1, b} /\ real{1} = real{2} /\ b{1} = real{1}).
+  call (_ : ={glob A1} ==> ={glob A1,res}); first by proc true.
+   wp ; rnd.  
+   by skip.
+ case (CSFE.OTSecurity.OTPSec.Protocol.validInputs i1{1} i2{2}).
+  rcondf {1} 1; first by move => &m0; skip.
+  rcondf {2} 1.
+   move => &m0;skip;move => &hr H.
+   move : H;delta;beta => H.
+   progress. smt. left. elim H. move => ? [[?]] ? ?. admit. idtac=>/#.
+  case (real{1}).
+   rcondt {1} 1; first by move => &m0; skip.
+   rcondt {2} 1; first by move => &m0; skip.
+   wp. call (_ : ={glob A1,view} ==> ={glob A1,res}); first by proc true.
+   wp; call SomeOT.R2_stateless; call SomeOT.R1_stateless.
+   skip;progress;smt.
+  rcondf {1} 1; first by move => &m0; skip.
+  rcondf {2} 1; first by move => &m0; skip.
+  wp. call (_ : ={glob A1,view} ==> ={glob A1,res}); first by proc true.
+  wp; call SomeOT.S1_stateless.
+  wp;skip;progress;smt.
+ rcondt {1} 1; first by move => &m0; skip.
+ rcondt {2} 1. move => &m0; skip. progress. move : H. simplify CSFE.OTSecurity.OTPSec.Protocol.validInputs. simplify SomeOT.OTSecurity.OTPSec.Protocol.validInputs. progress. admit.
+ wp;rnd;skip;progress;smt.
+ qed.
+
+ lemma Connect_SomeOT_1_pr : 
+  forall (A1 <: CSFE.OTSecurity.OTPSec.Adv1_t) &m,
+   islossless A1.gen_query =>
+   islossless A1.dist =>
+   Pr[CSFE.OTSecurity.OTPSec.Game1(SomeOT.R1, SomeOT.R2, SomeOT.S, A1).main() @ &m : res] =
+   Pr[SomeOT.OTSecurity.OTPSec.Game1(SomeOT.R1, SomeOT.R2, SomeOT.S, A1).main() @ &m : res].
+ proof strict.
+ move => A1 &m A1genll A1getll.
+ by byequiv (Connect_SomeOT_1 A1 &m _ _).
+ qed.
+
+ lemma Connect_SomeOT_2 : 
+  forall (A2 <: CSFE.OTSecurity.OTPSec.Adv2_t) &m,
+   islossless A2.gen_query =>
+   islossless A2.dist =>
+   equiv [ CSFE.OTSecurity.OTPSec.Game2(SomeOT.R1, SomeOT.R2, SomeOT.S, A2).main ~
+           SomeOT.OTSecurity.OTPSec.Game2(SomeOT.R1, SomeOT.R2, SomeOT.S, A2).main : 
+           ={glob A2} ==> ={res} ].
+ proof strict.
+ move => A2 &m A2genll A2distll; proc.
+ inline CSFE.OTSecurity.OTPSec.Game2(SomeOT.R1, SomeOT.R2, SomeOT.S, A2).game.
+ inline SomeOT.OTSecurity.OTPSec.Game2(SomeOT.R1, SomeOT.R2, SomeOT.S, A2).game.
+ seq 3 3 : (={i1,i2,glob A2,b} /\ real{1} = real{2} /\ b{1} = real{1}).
+  call (_ : ={glob A2} ==> ={glob A2,res}); first by proc true.
+  wp; rnd; by skip.
+ case (CSFE.OTSecurity.OTPSec.Protocol.validInputs i1{1} i2{2}).
+  rcondf {1} 1; first by move => &m0; skip.
+  rcondf {2} 1.
+   move => &m0; skip; move => &hr H.
+   move : H;delta;beta => H.
+   progress;admit. 
+  case (real{1}).
+   rcondt {1} 1; first by move => &m0; skip.
+   rcondt {2} 1; first by move => &m0; skip.
+   wp. call (_ : ={glob A2,view} ==> ={glob A2,res}); first by proc true.
+   wp; call SomeOT.R2_stateless; call SomeOT.R1_stateless.
+   skip; progress; smt.
+  rcondf {1} 1; first by move => &m0; skip.
+  rcondf {2} 1; first by move => &m0; skip.
+  wp. call (_ : ={glob A2,view} ==> ={glob A2,res}); first by proc true.
+  wp; call SomeOT.S2_stateless.
+  wp; skip; progress; smt.
+ rcondt {1} 1; first by move => &m0; skip.
+ wp. rcondt {2} 1; first by move => &m0; skip; admit.
+ rnd; wp; skip; progress; smt.
+ qed.
+
+ lemma Connect_SomeOT_2_pr : 
+  forall (A2 <: CSFE.OTSecurity.OTPSec.Adv2_t) &m,
+    islossless A2.gen_query =>
+    islossless A2.dist =>
+     Pr[CSFE.OTSecurity.OTPSec.Game2(SomeOT.R1, SomeOT.R2, SomeOT.S, A2).main() @ &m : res] = Pr[SomeOT.OTSecurity.OTPSec.Game2(SomeOT.R1, SomeOT.R2, SomeOT.S, A2).main() @ &m : res].
+ proof strict.
+ move => A2 &m A2genll A2getll.
+ by byequiv (Connect_SomeOT_2 A2 &m _ _).
+ qed.
+
+ lemma Connect_SomeGarble : 
+  forall (A <: CSFE.SchSecurity.EncSecurity.Adv_SIM_t) &m,
+   islossless A.gen_query =>
+   islossless A.get_challenge =>
+   equiv [ CSFE.SchSecurity.EncSecurity.Game_SIM(ES.Rand, ES.SchSecurity.EncSecurity.SIM(ES.Rand), A).main ~
+           ES.SchSecurity.EncSecurity.Game_SIM(ES.Rand, ES.SchSecurity.EncSecurity.SIM(ES.Rand), A).main :
+           ={glob A} ==> ={res}  ].
+ proof strict.
+ move => A &m Agenll Agetll; proc.
+ inline CSFE.SchSecurity.EncSecurity.Game_SIM(ES.Rand, ES.SchSecurity.EncSecurity.SIM(ES.Rand), A).game.
+ inline ES.SchSecurity.EncSecurity.Game_SIM(ES.Rand, ES.SchSecurity.EncSecurity.SIM(ES.Rand), A).game.
+   wp; seq 3 3 : (={glob A,query, b} /\ real{1} = real{2} /\ b{1} = real{1}).
+  call (_ : ={glob A} ==> ={glob A,res}); first by proc true.
+  wp;rnd. by skip.
+ case (CSFE.SchSecurity.EncSecurity.queryValid_SIM query{1}).
+  rcondf {1} 1; first by move =>  &m0; skip.
+  rcondf {2} 1; first by move =>  &m0; skip; smt.
+  case (real{1}).
+   rcondt {1} 1; first by move =>  &m0; skip.
+   rcondt {2} 1; first by move =>  &m0; skip.
+   call (_ : ={glob A,cipher} ==> ={res,glob A}); first by proc true.
+   wp; call ES.Rand_stateless.
+   skip;progress;smt.
+  rcondf {1} 1; first by move =>  &m0; skip.
+  rcondf {2} 1; first by move =>  &m0; skip.
+  call (_ : ={glob A,cipher} ==> ={res,glob A}); first by proc true.
+  inline ES.SchSecurity.EncSecurity.SIM(ES.Rand).simm.
+  wp; call ES.Rand_stateless.
+  wp;skip;progress;smt.
+ rcondt {1} 1; first by move =>  &m0; skip.
+ rcondt {2} 1; first by move =>  &m0; skip; smt.
+ rnd;wp;skip;smt.
+ qed.
+
+ lemma Connect_SomeGarble_pr : 
+  forall (A <: CSFE.SchSecurity.EncSecurity.Adv_SIM_t) &m,
+   islossless A.gen_query =>
+   islossless A.get_challenge =>
+   Pr[CSFE.SchSecurity.EncSecurity.Game_SIM(ES.Rand, ES.SchSecurity.EncSecurity.SIM(ES.Rand), A).main() @ &m : res ] =
+   Pr[ES.SchSecurity.EncSecurity.Game_SIM(ES.Rand, ES.SchSecurity.EncSecurity.SIM(ES.Rand), A).main() @ &m : res].
+ proof strict.
+ move => A &m Agenll Agetll.
+ by byequiv (Connect_SomeGarble A &m _ _).
+ qed.
+
+ print SomeOT.ot_correct.
+ 
+ lemma Connect_SFE : 
+ forall (PFE_A1<:CSFE.ProtSecurity.Adv1_t {SomeOT.R1, SomeOT.R2, SomeOT.S,ES.Rand, ES.SchSecurity.EncSecurity.SIM, CSFE.B_OT1, CSFE.B_G})
+        (PFE_A2<:CSFE.ProtSecurity.Adv2_t{SomeOT.R1, SomeOT.R2, SomeOT.S,ES.Rand, ES.SchSecurity.EncSecurity.SIM, CSFE.B_OT2, CSFE.B_G}) &m, 
+  islossless PFE_A1.gen_query => islossless PFE_A1.dist =>
+  islossless PFE_A2.gen_query => islossless PFE_A2.dist =>
+   `|2%r * Pr[CSFE.ProtSecurity.Game1(R1, R2, SFESim, PFE_A1).main()@ &m:res] - 1%r| <=
+     `|2%r * Pr[CSFE.OTSecurity.OTPSec.Game1(SomeOT.R1, SomeOT.R2, SomeOT.S, CSFE.B_OT1(ES.Rand, PFE_A1)).main() @ &m : res] - 1%r| +
+     `|2%r * Pr[CSFE.SchSecurity.EncSecurity.Game_SIM(ES.Rand, ES.SchSecurity.EncSecurity.SIM(ES.Rand), CSFE.B_G(SomeOT.S, PFE_A1)).main() @ &m : res] - 1%r| /\
+   `|2%r * Pr[CSFE.ProtSecurity.Game2(R1, R2, SFESim, PFE_A2).main()@ &m:res] - 1%r| <=
+     `|2%r * Pr[CSFE.OTSecurity.OTPSec.Game2(SomeOT.R1, SomeOT.R2, SomeOT.S, CSFE.B_OT2(ES.Rand, PFE_A2)).main() @ &m : res] - 1%r|.   
+ proof strict.
+move => A1 A2 &m A1_gen_ll A1_dist_ll A2_gen_ll A2_dist_ll.
+apply (CSFE.PFE_Security _ _ (SomeOT.R1) (SomeOT.R2) (SomeOT.S) (ES.Rand) (ES.SchSecurity.EncSecurity.SIM(ES.Rand)) A1 A2 &m _ _ _ _ _ _ _ _ _ _ _ _ _ _ _); trivial.
+ by apply compatible; smt. 
+ admit. trivial. trivial. (*by apply SomeOT.ot_correct.*)
+ by apply SomeOT.R1_lossless.
+ by apply SomeOT.R2_lossless.
+ by apply SomeOT.S1_lossless.
+ by apply SomeOT.S2_lossless.
+ by apply ES.Rand_islossless.
+proc; wp. 
+wp; call ES.Rand_islossless.
+wp => //.
+qed.
+
+ lemma Security : 
+  forall (A1 <: ProtSecurity.Adv1_t {ES.Rand, CSFE.B_OT1, CSFE.B_G, SomeOT.DDHn_A, SomeOT.ESn_A}) (A2 <: ProtSecurity.Adv2_t {ES.Rand, CSFE.B_OT2, CSFE.B_G}) &m,
+   islossless A1.gen_query =>
+   islossless A1.dist =>
+   islossless A2.gen_query =>
+   islossless A2.dist =>
+   let epsilon = `|2%r * Pr[SomeOT.ESn.Game(SomeOT.ESn_A(CSFE.B_OT1(ES.Rand ,SFE_A1(A1)))).main()@ &m:res] - 1%r| +
+                 `|2%r * Pr[DDH.DDHn.Game(SomeOT.DDHn_A(CSFE.B_OT1(ES.Rand, SFE_A1(A1)))).main() @ &m : res] - 1%r| +
+                 2%r * ((ES.SomeGarble.bound)%ES.SomeGarble + 1)%r *
+                  `|2%r * Pr[ES.SomeGarble.DKCSecurity.Game(ES.SomeGarble.DKCSecurity.DKC, ES.SomeGarble.Sec.EncSecurity.RedSI(ES.Red(CSFE.B_G(SomeOT.S, SFE_A1(A1))))).main() @ &m : res] - 1%r| in
+   `|2%r * Pr[ProtSecurity.Game1(R1, R2, S, A1).main() @ &m : res] - 1%r| <= epsilon /\
+   `|2%r * Pr[ProtSecurity.Game2(R1, R2, S, A2).main() @ &m : res] - 1%r| <= epsilon.
+   (* François: - We can replace epsilon by 0%r in the last line is it normal ? *)
+ proof strict.
+ intros A1 A2 &m A1genll A1distll A2genll A2distll bound.
+
+ cut Randgenll : islossless ES.Rand.gen by apply ES.Rand_islossless.
+ cut Ssim1ll : islossless SomeOT.S.sim1 by apply SomeOT.S1_lossless.
+ cut SFE_A1genll  : islossless SFE_A1(A1).gen_query by (fun; call A1genll; trivial).
+ cut SFE_A1distll : islossless SFE_A1(A1).dist      by (fun; call A1distll;trivial).
+ cut SFE_A2genll  : islossless SFE_A2(A2).gen_query by (fun; call A2genll; trivial).
+ cut SFE_A2distll : islossless SFE_A2(A2).dist      by (fun; call A2distll;trivial).
+ cut B_OT1_gen_ll : islossless CSFE.B_OT1(ES.Rand ,SFE_A1(A1)).gen_query
+  by (apply (CSFE.B_OT1_gen_ll ES.Rand (SFE_A1(A1)) _ _)=> //).
+ cut B_OT1_dist_ll : islossless CSFE.B_OT1(ES.Rand ,SFE_A1(A1)).dist
+  by (apply (CSFE.B_OT1_dist_ll ES.Rand (SFE_A1(A1)) _)=> //).
+ cut B_OT2_gen_ll : islossless CSFE.B_OT2(ES.Rand ,SFE_A2(A2)).gen_query
+  by (apply (CSFE.B_OT2_gen_ll ES.Rand (SFE_A2(A2)) _ _)=> //).
+ cut B_OT2_dist_ll : islossless CSFE.B_OT2(ES.Rand ,SFE_A2(A2)).dist
+  by (apply (CSFE.B_OT2_dist_ll ES.Rand (SFE_A2(A2)) _)=> //).
+ cut B_G_gen_ll : islossless CSFE.B_G(SomeOT.S, SFE_A1(A1)).gen_query
+  by (apply (CSFE.B_G_gen_ll SomeOT.S (SFE_A1(A1)) _)=> //).
+ cut B_G_dist_ll : islossless CSFE.B_G(SomeOT.S, SFE_A1(A1)).get_challenge
+  by (apply (CSFE.B_G_dist_ll SomeOT.S (SFE_A1(A1)) _)=> //).
+
+ elim (Connect_SFE (SFE_A1(A1)) (SFE_A2(A2)) &m _ _ _ _)=> //.
+ elim (SomeOT.ot_is_sec (CSFE.B_OT1(ES.Rand ,SFE_A1(A1))) (CSFE.B_OT2(ES.Rand ,SFE_A2(A2))) &m _ _ _ _
+  `|2%r * Pr[SomeOT.ESn.Game(SomeOT.ESn_A(CSFE.B_OT1(ES.Rand ,SFE_A1(A1)))).main() @ &m : res] - 1%r|
+  `|2%r * Pr[DDH.DDHn.Game(SomeOT.DDHn_A(CSFE.B_OT1(ES.Rand, SFE_A1(A1)))).main() @ &m : res] - 1%r| _ _)=> //.
+ cut := ES.sch_is_sim  (CSFE.B_G(SomeOT.S, SFE_A1(A1))) &m _ _=> //.
+
+ rewrite (Connect_DKCScheme_pr (CSFE.B_G(SomeOT.S, SFE_A1(A1))) &m) //.
+ rewrite (Connect_SFE_2_pr (A2) &m) // (Connect_SFE_1_pr (A1) &m) //.
+ rewrite (Connect_SomeOT_1_pr (CSFE.B_OT1(ES.Rand ,SFE_A1(A1))) &m) //.
+ rewrite (Connect_SomeOT_2_pr (CSFE.B_OT2(ES.Rand ,SFE_A2(A2))) &m) //.
+
+ rewrite /bound.
+
+ clear A1genll A1distll A2genll A2distll bound Randgenll Ssim1ll SFE_A1genll SFE_A1distll SFE_A2genll
+   SFE_A2distll B_OT1_gen_ll B_OT1_dist_ll B_OT2_gen_ll B_OT2_dist_ll B_G_gen_ll B_G_dist_ll.
+
+ progress;smt.
+ qed.
